![[Pasted image 20250416134752.png|625]]
对于$R_1$，1=0+1，2=1+1，3=2+1，1=2/2，0=0/2，$R_1=\{(0, 1), (1, 2), (2, 3), (2, 1), (0, 0)\}$
对于$R_2$，2=0+2，3=1+2，$R_2=\{(2, 0), (3, 1)\}$

(1) 设$(a, c)∈ R_1∘R_2$，则 $(a, b)∈R_1，(b,c)∈R_2$，可得 $R_1∘R_2 = \{(1, 0), (2, 1)\}$
(2)设$(a, c)∈ R_2∘R_1$，则 $(a, b)∈R_2，(b,c)∈R_1$，可得 $R_2∘R_1 = \{(2, 1), (2, 0), (3, 2)\}$
(3)由(1)得$R_1∘R_2 = \{(1, 0), (2, 1)\}$，则$R_1∘R_2∘R_1= \{(1, 1), (1, 0), (2, 2)\}$

---
![[Pasted image 20250416140123.png|625]]
(1) $R_1, R_2$对称，则
	设$(c, a)∈R_2∘R_1$，则存在$(c,b)∈R_2$，$(b,a)∈R_1$
	由对称性，则$(b,c)∈R_2，(a,b)∈R_1$
	故$(a, c)∈ R_1∘R_2$；又$R_1∘R_2⊆R_2∘R_1$，所以$(a, c)∈ R_2∘R_1$
	因此$R_1∘R_2$满足对称性
	又$R_1∘R_2⊆R_2∘R_1$，
	则$R_1∘R_2 = R_2∘R_1$
(2)$(a,a)\in R$，$(b,b)\in S$
	设b=a，则$(a,b) = (a,a) \in R , (b,a) = (a,a) \in S$
	则$(a,a) \in R∘S$

---
![[Pasted image 20250416144953.png|625]]
自反性：
	设a=c, d=b，ad=ab=bc=ba
	(a,b)~(a,b)
对称性：
	若(a,b)~(c,d)，则ad=bc
	则cb=da
	(c,d)~(a,b)
传递性：
	若(a,b)~(c,d), (c,d)~(e,f)
	则ad=bc，cf=ed
	a/b=c/d=e/f
	则af=be
	所以(a,b)~(e,f)
	即(a,b)~(c,d)∧(c,d)~(e,f)→(a,b)~(e,f)
综上，~是等价关系

---
![[Pasted image 20250416145657.png|625]]
(1)
- 对于1，$(1,1)∈R, (1,5)(5,1) \in R, [1]={1,5}$
- 对于2，$(2,2) \in R, (2,3)(3,2) \in R, (2,6)(6,2) \in R, [2]={2,3,6}$
- 对于4，$(4,4) \in R, [4]={4}$
(2)
	-同等价类， {{1,5}, {2,3,6}, {4}}
	- {{1,2,3}, {4}, {5}, {6}}
	- {{1,2}, {3,4}, {5}, {6}}
	- {{1}, {2}, {3}, {4,5,6}}

---
![[Pasted image 20250416150415.png|525]]
(a)

|     | a   | b   | c   |
| --- | --- | --- | --- |
| a   | 1   | 1   | 1   |
| b   | 1   | 0   | 0   |
| c   | 1   | 0   | 0   |
对称关系
(b)

|     | a   | b   | c   |
| --- | --- | --- | --- |
| a   | 0   | 1   | 0   |
| b   | 0   | 0   | 0   |
| c   | 1   | 0   | 0   |
反自反关系、反对称关系
(c)

|     | a   | b   | c   |
| --- | --- | --- | --- |
| a   | 1   | 0   | 1   |
| b   | 1   | 1   | 0   |
| c   | 0   | 1   | 1   |
自反关系、反对称关系