![[Pasted image 20250401211546.png|174]]
(1) ρ({a,{a}}) = {∅, {a}, {{a}}, {a,{a}}}
(2) ρ({∅,a,{a}}) = {∅, {∅}, {a}, {{a}}, {∅,a}, {∅, {a}}, {a,{a}}, {∅,a,{a}}}
(3) ρ({1, 2, 3, 4}) = {∅, {1}, {2}, {3}, {4}, {1,2}, {1,3}, {1,4}, {2,3}, {2,4}, {3,4}, {1,2,3}, {1,2,4}, {1,3,4}, {2,3,4}, {1,2,3,4}}

![[Pasted image 20250401212315.png||200]]
(1) A×B = {(0,1), (0,2), (1,1), (1,2)}
(2) A²×B = A×A×B = {(0,0), (0,1), (1,1), (1,0)}×B
	 = {((0,0),1), ((0,1),1), ((1,0),1), ((1,1),1), ((0,0),2), ((0,1),2), ((1,0),2), ((1,1),2)}
(3) B×A = {(1,0), (1,1), (2,0), (2,1)}

![[Pasted image 20250401213012.png|425]]
(1)正确。∀x(x∈B)→x∈C，又A∈B，所以A∈C
(2)不正确。若A = ∅，A⊆C成立；若A不等于∅，对于{x | x∈A∧x∉B}，x∉C，则A⊊C
(3)不正确。A∈C当且仅当A = B。如A = {1}, B = {1,2}, C = {{1,2}, 3}, A∉C
(4)不正确。如A = {1}, B = {1,2}, C = {{1,2}, 3}, A⊊C

![[Pasted image 20250401214242.png|275]]
(1)
- A∩(B-C) = A∩(B∩~C)
- (A∩B)−(A∩C) = (A∩B)∩~(A∩C) = (A∩B)∩(~A∪~C)
	 = (A∩B∩~A)∪(A∩B∩~C) = A∩(B∩~C) = A∩(B-C)
- ∴A∩(B-C) = (A∩B)−(A∩C)
(2)
- (A-B)-C = A∩~B∩~C
- A-(B∪C) = A∩~(B∪C) = A∩(~B∩~C) = A∩~B∩~C = (A-B)-C
- ∴(A-B)-C = A-(B∪C)
